rename rec_heap_inj -> rec_heap_bij2

dimsum_examples/rec_heap_bij2.v
@@ -8,24 +8,24 @@ From dimsum.examples Require Export heapUR.
 
 Set Default Proof Using "Type".
 
-(** * rec_heap_inj *)
-(** [rec_heap_inj] allows injections of memory when proving a
+(** * rec_heap_bij *)
+(** [rec_heap_bij] allows bijections of memory when proving a
 refinement between two Rec modules. *)
 
 (** * Camera definition *)
-Definition heap_injUR : ucmra :=
+Definition heap_bijUR : ucmra :=
   prodUR (optionO (agree (gset prov)))
  (prodUR (gmap_viewUR prov (agreeR locO))
  (prodUR heapUR
  (heapUR))).
 
-Global Instance heap_injUR_shrink : Shrink heap_injUR.
+Global Instance heap_bijUR_shrink : Shrink heap_bijUR.
 Proof. solve_shrink. Qed.
 
-Global Instance heap_injUR_discrete : CmraDiscrete heap_injUR.
+Global Instance heap_bijUR_discrete : CmraDiscrete heap_bijUR.
 Proof. apply _. Qed.
 
-Program Definition own_heap_s : BiOwn (uPredI heap_injUR) heapUR := {|
+Program Definition own_heap_s : BiOwn (uPredI heap_bijUR) heapUR := {|
   bi_own r := uPred_ownM (None, (ε, (r, ε)))
 |}.
 Next Obligation.
@@ -39,7 +39,7 @@ Next Obligation.
 Qed.
 Next Obligation. solve_proper. Qed.
 
-Program Definition own_heap_i : BiOwn (uPredI heap_injUR) heapUR := {|
+Program Definition own_heap_i : BiOwn (uPredI heap_bijUR) heapUR := {|
   bi_own r := uPred_ownM (None, (ε, (ε, r)))
 |}.
 Next Obligation.
@@ -53,25 +53,25 @@ Next Obligation.
 Qed.
 Next Obligation. solve_proper. Qed.
 
-Definition heap_injUR_statics_inj (r : agree (gset prov)) : heap_injUR := ((Some r), (ε, ε)).
-Definition heap_injUR_shared_inj (r : (gmap_viewUR prov (agreeR locO))) : heap_injUR
+Definition heap_bijUR_statics_inj (r : agree (gset prov)) : heap_bijUR := ((Some r), (ε, ε)).
+Definition heap_bijUR_shared_inj (r : (gmap_viewUR prov (agreeR locO))) : heap_bijUR
   := (None, (r, ε)).
 
 
 (** * ghost theory *)
 (** ** Ghost state definitions *)
-Definition heap_inj_shared_auth_raw (ps : gmap prov loc) : uPred (heap_injUR) :=
-  uPred_ownM (heap_injUR_shared_inj $ gmap_view_auth (DfracOwn 1) (to_agree <$> ps)).
-Definition heap_inj_shared (ps : prov) (li : loc) : uPred (heap_injUR) :=
-  uPred_ownM (heap_injUR_shared_inj $ gmap_view_frag ps DfracDiscarded (to_agree li)).
-Definition heap_inj_statics (provs : gset prov) :=
-  uPred_ownM (heap_injUR_statics_inj (to_agree provs)).
+Definition heap_bij_shared_auth_raw (ps : gmap prov loc) : uPred (heap_bijUR) :=
+  uPred_ownM (heap_bijUR_shared_inj $ gmap_view_auth (DfracOwn 1) (to_agree <$> ps)).
+Definition heap_bij_shared (ps : prov) (li : loc) : uPred (heap_bijUR) :=
+  uPred_ownM (heap_bijUR_shared_inj $ gmap_view_frag ps DfracDiscarded (to_agree li)).
+Definition heap_bij_statics (provs : gset prov) :=
+  uPred_ownM (heap_bijUR_statics_inj (to_agree provs)).
 
-Definition heap_inj_shared_auth (ps : gmap prov loc) : uPred (heap_injUR) :=
-  heap_inj_shared_auth_raw ps ∗ [∗ map] ps↦li0∈ps, heap_inj_shared ps li0.
+Definition heap_bij_shared_auth (ps : gmap prov loc) : uPred (heap_bijUR) :=
+  heap_bij_shared_auth_raw ps ∗ [∗ map] ps↦li0∈ps, heap_bij_shared ps li0.
 
-Notation heap_inj_inv_s := (heapUR_inv own_heap_s).
-Notation heap_inj_inv_i := (heapUR_inv own_heap_i).
+Notation heap_bij_inv_s := (heapUR_inv own_heap_s).
+Notation heap_bij_inv_i := (heapUR_inv own_heap_i).
 
 Notation "l '↦hs' dq v" := (heapUR_ptsto own_heap_s l dq v)
   (at level 20, dq custom dfrac, format "l  ↦hs dq  v") : bi_scope.
@@ -89,9 +89,9 @@ Notation "p '↦∗hi' dq b" := (heapUR_block own_heap_i p dq b)
   (at level 20, dq custom dfrac at level 1, format "p  '↦∗hi' dq  b") : bi_scope.
 
 (** ** Ghost state lemmas *)
-Lemma heap_inj_statics_eq h1 h2 :
-  heap_inj_statics h1 -∗
-  heap_inj_statics h2 -∗
+Lemma heap_bij_statics_eq h1 h2 :
+  heap_bij_statics h1 -∗
+  heap_bij_statics h2 -∗
   ⌜h1 = h2⌝.
 Proof.
   apply bi.wand_intro_r. apply bi.wand_intro_r. rewrite left_id. rewrite -uPred.ownM_op.
@@ -100,10 +100,10 @@ Proof.
   by fold_leibniz.
 Qed.
 
-Lemma heap_inj_shared_alloc_raw ps li0 inj :
-  inj !! ps = None →
-  heap_inj_shared_auth_raw inj ⊢ |==>
-  heap_inj_shared_auth_raw (<[ps := li0]>inj) ∗ heap_inj_shared ps li0.
+Lemma heap_bij_shared_alloc_raw ps li0 bij :
+  bij !! ps = None →
+  heap_bij_shared_auth_raw bij ⊢ |==>
+  heap_bij_shared_auth_raw (<[ps := li0]>bij) ∗ heap_bij_shared ps li0.
 Proof.
   move => ?. rewrite -uPred.ownM_op. apply uPred.bupd_ownM_update.
   apply prod_update; [done|] => /=. apply prod_update; [|done] => /=.
@@ -111,19 +111,19 @@ Proof.
   by rewrite lookup_fmap fmap_None.
 Qed.
 
-Lemma heap_inj_shared_alloc ps li0 inj :
-  inj !! ps = None →
-  heap_inj_shared_auth inj ⊢ |==>
-  heap_inj_shared_auth (<[ps := li0]>inj) ∗ heap_inj_shared ps li0.
+Lemma heap_bij_shared_alloc ps li0 bij :
+  bij !! ps = None →
+  heap_bij_shared_auth bij ⊢ |==>
+  heap_bij_shared_auth (<[ps := li0]>bij) ∗ heap_bij_shared ps li0.
 Proof.
-  iIntros (?) "[??]". iMod (heap_inj_shared_alloc_raw with "[$]") as "[$ #$]"; [done|].
+  iIntros (?) "[??]". iMod (heap_bij_shared_alloc_raw with "[$]") as "[$ #$]"; [done|].
   iModIntro. by iApply big_sepM_insert_2.
 Qed.
 
-Lemma heap_inj_shared_lookup_raw ps li0 inj  :
-  heap_inj_shared_auth_raw inj -∗
-  heap_inj_shared ps li0 -∗
-  ⌜inj !! ps = Some li0⌝.
+Lemma heap_bij_shared_lookup_raw ps li0 bij  :
+  heap_bij_shared_auth_raw bij -∗
+  heap_bij_shared ps li0 -∗
+  ⌜bij !! ps = Some li0⌝.
 Proof.
   apply bi.wand_intro_r. apply bi.wand_intro_r. rewrite left_id.
   rewrite -uPred.ownM_op. etrans; [apply uPred.ownM_valid|].
@@ -133,79 +133,79 @@ Proof.
   move => /to_agree_included_L. naive_solver.
 Qed.
 
-Lemma heap_inj_shared_lookup ps li0 inj  :
-  heap_inj_shared_auth inj -∗
-  heap_inj_shared ps li0 -∗
-  ⌜inj !! ps = Some li0⌝.
-Proof. iIntros "[? _]". by iApply heap_inj_shared_lookup_raw. Qed.
+Lemma heap_bij_shared_lookup ps li0 bij  :
+  heap_bij_shared_auth bij -∗
+  heap_bij_shared ps li0 -∗
+  ⌜bij !! ps = Some li0⌝.
+Proof. iIntros "[? _]". by iApply heap_bij_shared_lookup_raw. Qed.
 
-Lemma heap_inj_shared_lookup_big inj' inj  :
-  heap_inj_shared_auth inj -∗
-  ([∗map] ps↦li0∈inj', heap_inj_shared ps li0) -∗
-  ⌜inj' ⊆ inj⌝.
+Lemma heap_bij_shared_lookup_big bij' bij  :
+  heap_bij_shared_auth bij -∗
+  ([∗map] ps↦li0∈bij', heap_bij_shared ps li0) -∗
+  ⌜bij' ⊆ bij⌝.
 Proof.
-  iIntros "Ha Hl". iInduction inj' as [|] "IH" using map_ind.
+  iIntros "Ha Hl". iInduction bij' as [|] "IH" using map_ind.
   { iPureIntro. apply map_empty_subseteq. }
   iDestruct (big_sepM_insert with "Hl") as "[??]"; [done|].
   iDestruct ("IH" with "[$] [$]") as %?.
-  iDestruct (heap_inj_shared_lookup with "Ha [$]") as %?.
+  iDestruct (heap_bij_shared_lookup with "Ha [$]") as %?.
   iPureIntro. by apply insert_subseteq_l.
 Qed.
 
-Lemma heap_inj_shared_alloc_big_raw inj inj' :
-  inj ⊆ inj' →
-  heap_inj_shared_auth inj ⊢ |==>
-  heap_inj_shared_auth inj'.
+Lemma heap_bij_shared_alloc_big_raw bij bij' :
+  bij ⊆ bij' →
+  heap_bij_shared_auth bij ⊢ |==>
+  heap_bij_shared_auth bij'.
 Proof.
-  iIntros (Hsub) "?". rewrite -(map_difference_union inj inj') //.
-  have Hdisj : (inj ##ₘ inj' ∖ inj) by apply map_disjoint_difference_r'.
+  iIntros (Hsub) "?". rewrite -(map_difference_union bij bij') //.
+  have Hdisj : (bij ##ₘ bij' ∖ bij) by apply map_disjoint_difference_r'.
   rewrite map_union_comm //.
-  iInduction (inj' ∖ inj) as [|] "IH" using map_ind forall (Hdisj).
+  iInduction (bij' ∖ bij) as [|] "IH" using map_ind forall (Hdisj).
   { by rewrite left_id_L. }
   move: Hdisj => /map_disjoint_insert_r[??].
   iMod ("IH" with "[%] [$]") as "?"; [done|].
   rewrite -insert_union_l.
-  iMod (heap_inj_shared_alloc with "[$]") as "[$ _]". 2: done.
+  iMod (heap_bij_shared_alloc with "[$]") as "[$ _]". 2: done.
   by apply lookup_union_None.
 Qed.
 
-Lemma heap_inj_shared_alloc_big inj inj' :
-  inj ⊆ inj' →
-  heap_inj_shared_auth inj ⊢ |==>
-  heap_inj_shared_auth inj' ∗ [∗ map] ps↦li0∈inj', heap_inj_shared ps li0.
+Lemma heap_bij_shared_alloc_big bij bij' :
+  bij ⊆ bij' →
+  heap_bij_shared_auth bij ⊢ |==>
+  heap_bij_shared_auth bij' ∗ [∗ map] ps↦li0∈bij', heap_bij_shared ps li0.
 Proof.
   iIntros (Hsub) "?".
-  iMod (heap_inj_shared_alloc_big_raw with "[$]") as "[? ?]"; [done|].
+  iMod (heap_bij_shared_alloc_big_raw with "[$]") as "[? ?]"; [done|].
   iModIntro. iSplit!. iFrame.
 Qed.
 
-Lemma heap_inj_shared_auth_shared inj :
-  heap_inj_shared_auth inj ⊢ [∗ map] ps↦li0∈inj, heap_inj_shared ps li0.
+Lemma heap_bij_shared_auth_shared bij :
+  heap_bij_shared_auth bij ⊢ [∗ map] ps↦li0∈bij, heap_bij_shared ps li0.
 Proof. iIntros "[? $]". Qed.
 
-Global Typeclasses Opaque heap_inj_shared_auth.
+Global Typeclasses Opaque heap_bij_shared_auth.
 
-(** * val_in_inj *)
-Definition loc_in_inj (li ls : loc) : uPred heap_injUR :=
-  ∃ li0, ⌜li = li0 +ₗ ls.2⌝ ∗ heap_inj_shared ls.1 li0.
+(** * val_in_bij *)
+Definition loc_in_bij (li ls : loc) : uPred heap_bijUR :=
+  ∃ li0, ⌜li = li0 +ₗ ls.2⌝ ∗ heap_bij_shared ls.1 li0.
 
-Global Instance loc_in_inj_Persistent li ls : Persistent (loc_in_inj li ls).
+Global Instance loc_in_bij_Persistent li ls : Persistent (loc_in_bij li ls).
 Proof. apply _. Qed.
 
-Definition val_in_inj (vi vs : val) : uPred heap_injUR :=
+Definition val_in_bij (vi vs : val) : uPred heap_bijUR :=
   match vi, vs with
   | ValNum n1, ValNum n2 => ⌜n1 = n2⌝
   | ValBool b1, ValBool b2 => ⌜b1 = b2⌝
   | ValFn f1, ValFn f2 => ⌜f1 = f2⌝
-  | ValLoc l1, ValLoc l2 => loc_in_inj l1 l2
+  | ValLoc l1, ValLoc l2 => loc_in_bij l1 l2
   | _, _ => False
   end.
 
-Global Instance val_in_inj_Persistent vi vs : Persistent (val_in_inj vi vs).
+Global Instance val_in_bij_Persistent vi vs : Persistent (val_in_bij vi vs).
 Proof. destruct vi, vs => /=; apply _. Qed.
 
 Lemma big_sepL2_ValNum_inv_r vl zl :
-  ([∗ list] y1;y2 ∈ vl;(ValNum <$> zl), val_in_inj y1 y2) -∗
+  ([∗ list] y1;y2 ∈ vl;(ValNum <$> zl), val_in_bij y1 y2) -∗
   ⌜vl = (ValNum <$> zl)⌝.
 Proof.
   iIntros "Hvl".
@@ -217,19 +217,19 @@ Proof.
   naive_solver.
 Qed.
 
-Lemma eval_binop_inj o v1 v2 v1' v2' v:
+Lemma eval_binop_bij o v1 v2 v1' v2' v:
   eval_binop o v1 v2 = Some v →
-  val_in_inj v1' v1 -∗
-  val_in_inj v2' v2 -∗
-  ∃ v', ⌜eval_binop o v1' v2' = Some v'⌝ ∗ val_in_inj v' v.
+  val_in_bij v1' v1 -∗
+  val_in_bij v2' v2 -∗
+  ∃ v', ⌜eval_binop o v1' v2' = Some v'⌝ ∗ val_in_bij v' v.
 Proof.
   iIntros (?) "??".
-  destruct o, v1, v2, v1', v2' => //= *; unfold loc_in_inj; iDestruct!; iSplit!; unfold loc_in_inj; iSplit!.
+  destruct o, v1, v2, v1', v2' => //= *; unfold loc_in_bij; iDestruct!; iSplit!; unfold loc_in_bij; iSplit!.
   2: done. apply offset_loc_assoc.
 Qed.
 
-(** * heap_in_inj *)
-(* TODO: make this actually an injection. See
+(** * heap_in_bij *)
+(* TODO: make this an injection. See
 b611b0e2cb0e6c903638048347ff51d618f995f6 for a version that is not
 vertically compositional. Try the following version that should be vertically
 compositional (note the 1/2 fraction for the dom):
@@ -241,129 +241,129 @@ Definition heap_in_inj_inv (inj : gmap prov loc) (rem : list prov) :
       [∗ map] o∈d, ∃ vi vs, (li0 +ₗ o) ↦hi vi ∗ (p, o) ↦hs vs ∗ val_in_inj vi vs.
 
  *)
-Definition heap_in_inj_inv (inj : gmap prov loc) (rem : list prov) :
-  uPred heap_injUR :=
-    [∗ map] ps↦li0∈inj, ⌜ps ∈ rem⌝ ∨
+Definition heap_in_bij_inv (bij : gmap prov loc) (rem : list prov) :
+  uPred heap_bijUR :=
+    [∗ map] ps↦li0∈bij, ⌜ps ∈ rem⌝ ∨
       ∃ bi bs, ⌜li0.2 = 0%Z⌝ ∗ li0.1 ↦∗hi bi ∗ ps ↦∗hs bs ∗
-      [∗ map] o↦vi;vs∈bi;bs, val_in_inj vi vs.
+      [∗ map] o↦vi;vs∈bi;bs, val_in_bij vi vs.
 
-Definition heap_in_inj (rem : list prov) : uPred heap_injUR :=
-  ∃ inj, heap_inj_shared_auth inj ∗ heap_in_inj_inv inj rem.
+Definition heap_in_bij (rem : list prov) : uPred heap_bijUR :=
+  ∃ bij, heap_bij_shared_auth bij ∗ heap_in_bij_inv bij rem.
 
-Lemma heap_in_inj_inv_borrow ps li0 rem inj :
+Lemma heap_in_bij_inv_borrow ps li0 rem bij :
   ps ∉ rem →
-  inj !! ps = Some li0 →
-  heap_in_inj_inv inj rem -∗
-  ∃ bi bs, ⌜li0.2 = 0%Z⌝ ∗ heap_in_inj_inv inj (ps::rem) ∗
-  li0.1 ↦∗hi bi ∗ ps ↦∗hs bs ∗ [∗ map] o↦vi;vs∈bi;bs, val_in_inj vi vs.
+  bij !! ps = Some li0 →
+  heap_in_bij_inv bij rem -∗
+  ∃ bi bs, ⌜li0.2 = 0%Z⌝ ∗ heap_in_bij_inv bij (ps::rem) ∗
+  li0.1 ↦∗hi bi ∗ ps ↦∗hs bs ∗ [∗ map] o↦vi;vs∈bi;bs, val_in_bij vi vs.
 Proof.
-  iIntros (??) "Hinj".
-  iDestruct (big_sepM_lookup_acc_impl with "Hinj") as "[[%|[% [% [% $]]]] Hinj]";[done..|].
-  iSplit!. iApply "Hinj". 2: by iLeft; iPureIntro; set_solver.
+  iIntros (??) "Hbij".
+  iDestruct (big_sepM_lookup_acc_impl with "Hbij") as "[[%|[% [% [% $]]]] Hbij]";[done..|].
+  iSplit!. iApply "Hbij". 2: by iLeft; iPureIntro; set_solver.
   iIntros "!>" (????) "[%|$]". by iLeft; iPureIntro; set_solver.
 Qed.
 
-Lemma heap_in_inj_inv_split inj' inj :
-  inj' ⊆ inj →
-  heap_in_inj_inv inj [] ⊣⊢
-  heap_in_inj_inv inj' [] ∗ heap_in_inj_inv (inj ∖ inj') [].
+Lemma heap_in_bij_inv_split bij' bij :
+  bij' ⊆ bij →
+  heap_in_bij_inv bij [] ⊣⊢
+  heap_in_bij_inv bij' [] ∗ heap_in_bij_inv (bij ∖ bij') [].
 Proof.
-  move => ?. rewrite /heap_in_inj_inv -big_sepM_union ?map_difference_union//.
+  move => ?. rewrite /heap_in_bij_inv -big_sepM_union ?map_difference_union//.
   apply map_disjoint_difference_r'.
 Qed.
 
-Lemma heap_in_inj_inv_combine inj' inj :
-  heap_in_inj_inv inj [] -∗
-  heap_in_inj_inv inj' [] -∗
-  heap_in_inj_inv (inj ∪ inj') [].
+Lemma heap_in_bij_inv_combine bij' bij :
+  heap_in_bij_inv bij [] -∗
+  heap_in_bij_inv bij' [] -∗
+  heap_in_bij_inv (bij ∪ bij') [].
 Proof. apply: big_sepM_union_2. Qed.
 
-Lemma heap_in_inj_inv_return i ps bi bs li0 rem inj :
+Lemma heap_in_bij_inv_return i ps bi bs li0 rem bij :
   rem !! i = Some ps →
-  inj !! ps = Some li0 →
+  bij !! ps = Some li0 →
   li0.2 = 0%Z →
-  heap_in_inj_inv inj rem -∗
+  heap_in_bij_inv bij rem -∗
   li0.1 ↦∗hi bi -∗
   ps ↦∗hs bs -∗
-  ([∗ map] o↦vi;vs∈bi;bs, val_in_inj vi vs) -∗
-  heap_in_inj_inv inj (delete i rem).
+  ([∗ map] o↦vi;vs∈bi;bs, val_in_bij vi vs) -∗
+  heap_in_bij_inv bij (delete i rem).
 Proof.
-  iIntros (???) "Hinj Hi Hs Hvs".
-  iDestruct (big_sepM_lookup_acc_impl with "Hinj") as "[Hprev Hinj]";
+  iIntros (???) "Hbij Hi Hs Hvs".
+  iDestruct (big_sepM_lookup_acc_impl with "Hbij") as "[Hprev Hbij]";
     [done|].
-  iApply "Hinj".
+  iApply "Hbij".
   - iIntros "!>" (????) "[%Hin|$]". iLeft. iPureIntro.
     rewrite delete_take_drop. erewrite <-take_drop_middle in Hin; [|done].
     set_solver.
   - iRight. by iFrame.
 Qed.
 
-Lemma heap_in_inj_inv_return0 ps bi bs li0 rem inj :
-  inj !! ps = Some li0 →
+Lemma heap_in_bij_inv_return0 ps bi bs li0 rem bij :
+  bij !! ps = Some li0 →
   li0.2 = 0%Z →
-  heap_in_inj_inv inj (ps :: rem) -∗
+  heap_in_bij_inv bij (ps :: rem) -∗
   li0.1 ↦∗hi bi -∗
   ps ↦∗hs bs -∗
-  ([∗ map] o↦vi;vs∈bi;bs, val_in_inj vi vs) -∗
-  heap_in_inj_inv inj rem.
-Proof. iIntros (??) "????". by iApply (heap_in_inj_inv_return 0 with "[$] [$] [$]"). Qed.
+  ([∗ map] o↦vi;vs∈bi;bs, val_in_bij vi vs) -∗
+  heap_in_bij_inv bij rem.
+Proof. iIntros (??) "????". by iApply (heap_in_bij_inv_return 0 with "[$] [$] [$]"). Qed.
 
 
-Lemma heap_in_inj_init :
-  heap_inj_shared_auth ∅ -∗ heap_in_inj [].
+Lemma heap_in_bij_init :
+  heap_bij_shared_auth ∅ -∗ heap_in_bij [].
 Proof. iIntros "$". by iApply big_sepM_empty. Qed.
 
-Lemma heap_in_inj_borrow ps li0 rem :
+Lemma heap_in_bij_borrow ps li0 rem :
   ps ∉ rem →
-  heap_in_inj rem -∗
-  heap_inj_shared ps li0 -∗
-  ∃ bi bs, ⌜li0.2 = 0%Z⌝ ∗ heap_in_inj (ps :: rem) ∗
-  li0.1 ↦∗hi bi ∗ ps ↦∗hs bs ∗ [∗ map] o↦vi;vs∈bi;bs, val_in_inj vi vs.
+  heap_in_bij rem -∗
+  heap_bij_shared ps li0 -∗
+  ∃ bi bs, ⌜li0.2 = 0%Z⌝ ∗ heap_in_bij (ps :: rem) ∗
+  li0.1 ↦∗hi bi ∗ ps ↦∗hs bs ∗ [∗ map] o↦vi;vs∈bi;bs, val_in_bij vi vs.
 Proof.
-  iIntros (?) "[%inj [? Hinj]] Hsh".
-  iDestruct (heap_inj_shared_lookup with "[$] [$]") as %?.
-  iDestruct (heap_in_inj_inv_borrow with "[$]") as (???) "[$ [$ $]]" => //.
+  iIntros (?) "[%bij [? Hbij]] Hsh".
+  iDestruct (heap_bij_shared_lookup with "[$] [$]") as %?.
+  iDestruct (heap_in_bij_inv_borrow with "[$]") as (???) "[$ [$ $]]" => //.
   by iFrame.
 Qed.
 
-Lemma heap_in_inj_return i ps bi bs li0 rem :
+Lemma heap_in_bij_return i ps bi bs li0 rem :
   rem !! i = Some ps →
   li0.2 = 0%Z →
-  heap_in_inj rem -∗
-  heap_inj_shared ps li0 -∗
+  heap_in_bij rem -∗
+  heap_bij_shared ps li0 -∗
   li0.1 ↦∗hi bi -∗
   ps ↦∗hs bs -∗
-  ([∗ map] o↦vi;vs∈bi;bs, val_in_inj vi vs) -∗
-  heap_in_inj (delete i rem).
+  ([∗ map] o↦vi;vs∈bi;bs, val_in_bij vi vs) -∗
+  heap_in_bij (delete i rem).
 Proof.
-  iIntros (??) "[%inj [? Hinj]] Hsh Hi Hs Hvs".
-  iDestruct (heap_inj_shared_lookup with "[$] [$]") as %?.
-  iExists _. iFrame. by iApply (heap_in_inj_inv_return with "[$] [$] [$]").
+  iIntros (??) "[%bij [? Hbij]] Hsh Hi Hs Hvs".
+  iDestruct (heap_bij_shared_lookup with "[$] [$]") as %?.
+  iExists _. iFrame. by iApply (heap_in_bij_inv_return with "[$] [$] [$]").
 Qed.
 
-Lemma heap_in_inj_return0 ps bi bs li0 rem :
+Lemma heap_in_bij_return0 ps bi bs li0 rem :
   li0.2 = 0%Z →
-  heap_in_inj (ps :: rem) -∗
-  heap_inj_shared ps li0 -∗
+  heap_in_bij (ps :: rem) -∗
+  heap_bij_shared ps li0 -∗
   li0.1 ↦∗hi bi -∗
   ps ↦∗hs bs -∗
-  ([∗ map] o↦vi;vs∈bi;bs, val_in_inj vi vs) -∗
-  heap_in_inj rem.
-Proof. iIntros (?) "????". by iApply (heap_in_inj_return 0 with "[$] [$] [$] [$]"). Qed.
+  ([∗ map] o↦vi;vs∈bi;bs, val_in_bij vi vs) -∗
+  heap_in_bij rem.
+Proof. iIntros (?) "????". by iApply (heap_in_bij_return 0 with "[$] [$] [$] [$]"). Qed.
 
 
-Lemma heap_in_inj_range hi hs l1 l2 z rem:
+Lemma heap_in_bij_range hi hs l1 l2 z rem:
   l2.2 = 0%Z →
   heap_range hs l2 z →
   l2.1 ∉ rem →
-  heap_inj_inv_i hi -∗
-  heap_inj_inv_s hs -∗
-  heap_in_inj rem -∗
-  loc_in_inj l1 l2 -∗
+  heap_bij_inv_i hi -∗
+  heap_bij_inv_s hs -∗
+  heap_in_bij rem -∗
+  loc_in_bij l1 l2 -∗
   ⌜heap_range hi l1 z⌝.
 Proof.
   iIntros (? Hr ?) "Hinv1 Hinv2 ? [% [% ?]]". subst.
-  iDestruct (heap_in_inj_borrow with "[$] [$]") as (bi bs ?) "[?[?[??]]]"; [done|].
+  iDestruct (heap_in_bij_borrow with "[$] [$]") as (bi bs ?) "[?[?[??]]]"; [done|].
   iDestruct (heapUR_lookup_block with "Hinv1 [$]") as %<-.
   iDestruct (heapUR_lookup_block with "Hinv2 [$]") as %<-.
   iDestruct (big_sepM2_dom with "[$]") as %Heq.
@@ -373,37 +373,37 @@ Proof.
   by rewrite Heq Hr.
 Qed.
 
-Lemma heap_in_inj_lookup hi hs l1 l2 v rem:
+Lemma heap_in_bij_lookup hi hs l1 l2 v rem:
   h_heap hs !! l2 = Some v →
   l2.1 ∉ rem →
-  heap_inj_inv_i hi -∗
-  heap_inj_inv_s hs -∗
-  heap_in_inj rem -∗
-  loc_in_inj l1 l2 -∗
-  ∃ v', ⌜h_heap hi !! l1 = Some v'⌝ ∗ val_in_inj v' v.
+  heap_bij_inv_i hi -∗
+  heap_bij_inv_s hs -∗
+  heap_in_bij rem -∗
+  loc_in_bij l1 l2 -∗
+  ∃ v', ⌜h_heap hi !! l1 = Some v'⌝ ∗ val_in_bij v' v.
 Proof.
   iIntros (??) "Hinvi ? Hh [% [-> ?]]".
-  iDestruct (heap_in_inj_borrow with "[$] [$]") as (bi bs Hl0) "[?[?[??]]]"; [done|].
+  iDestruct (heap_in_bij_borrow with "[$] [$]") as (bi bs Hl0) "[?[?[??]]]"; [done|].
   iDestruct (heapUR_lookup_block1 with "[$] [$]") as %?; [done|].
   iDestruct (big_sepM2_lookup_r with "[$]") as (??) "$"; [done|].
   iDestruct (heapUR_lookup_block with "Hinvi [$]") as %<-.
   iPureIntro. by rewrite /offset_loc Hl0 Z.add_0_l -h_block_lookup.
 Qed.
 
-Lemma heap_in_inj_update h1 h2 l1 l2 v1 v2 rem:
+Lemma heap_in_bij_update h1 h2 l1 l2 v1 v2 rem:
   l2.1 ∉ rem →
   heap_alive h2 l2 →
-  heap_inj_inv_i h1 -∗
-  heap_inj_inv_s h2 -∗
-  heap_in_inj rem -∗
-  loc_in_inj l1 l2 -∗
-  val_in_inj v1 v2 ==∗
-  heap_inj_inv_i (heap_update h1 l1 v1) ∗
-  heap_inj_inv_s (heap_update h2 l2 v2) ∗
-  heap_in_inj rem.
+  heap_bij_inv_i h1 -∗
+  heap_bij_inv_s h2 -∗
+  heap_in_bij rem -∗
+  loc_in_bij l1 l2 -∗
+  val_in_bij v1 v2 ==∗
+  heap_bij_inv_i (heap_update h1 l1 v1) ∗
+  heap_bij_inv_s (heap_update h2 l2 v2) ∗
+  heap_in_bij rem.
 Proof.
-  iIntros (? [? Ha]) "Hinvi Hinvs Hinj [% [-> #?]] Hv".
-  iDestruct (heap_in_inj_borrow with "[$] [$]") as (bi bs Hli0) "[?[Hli[??]]]"; [done|].
+  iIntros (? [? Ha]) "Hinvi Hinvs Hbij [% [-> #?]] Hv".
+  iDestruct (heap_in_bij_borrow with "[$] [$]") as (bi bs Hli0) "[?[Hli[??]]]"; [done|].
   iDestruct (heapUR_lookup_block with "Hinvs [$]") as %<-.
   iDestruct (heapUR_lookup_block with "Hinvi [$]") as %<-.
   iMod (heapUR_update_in_block with "[$] [$]") as "[$ ?]"; [eexists _; done|].
@@ -412,98 +412,98 @@ Proof.
   iMod (heapUR_update_in_block with "[$] [Hli]") as "[$ ?]" => /=.
   { eexists _. by rewrite h_block_lookup2 /= Hli0 Z.add_0_l. } { done. }
   iModIntro. rewrite Hli0 Z.add_0_l.
-  iApply (heap_in_inj_return0 with "[$] [$] [$] [$]"); [done|].
+  iApply (heap_in_bij_return0 with "[$] [$] [$] [$]"); [done|].
   by iApply (big_sepM2_insert_2 with "[Hv] [$]").
 Qed.
 
-Lemma heap_in_inj_share li ls rem bi bs :
+Lemma heap_in_bij_share li ls rem bi bs :
   ls.1 ∉ rem →
   li.2 = 0%Z →
   ls.2 = 0%Z →
-  heap_in_inj rem -∗
+  heap_in_bij rem -∗
   li.1 ↦∗hi bi -∗
   ls.1 ↦∗hs bs -∗
-  ([∗ map] o↦vi;vs∈bi;bs, val_in_inj vi vs) ==∗
-  heap_in_inj rem ∗
-  loc_in_inj li ls.
+  ([∗ map] o↦vi;vs∈bi;bs, val_in_bij vi vs) ==∗
+  heap_in_bij rem ∗
+  loc_in_bij li ls.
 Proof.
-  iIntros (? ? Hl0) "[%inj[??]] ???".
-  destruct (inj !! ls.1) eqn:?. {
-    iDestruct (heap_in_inj_inv_borrow with "[$]") as (???) "[? [?[??]]]"; [done..|].
+  iIntros (? ? Hl0) "[%bij[??]] ???".
+  destruct (bij !! ls.1) eqn:?. {
+    iDestruct (heap_in_bij_inv_borrow with "[$]") as (???) "[? [?[??]]]"; [done..|].
     iDestruct (heapUR_block_excl with "[$] [$]") as %[]. }
-  iMod (heap_inj_shared_alloc with "[$]") as "[? #$]"; [done|]. iModIntro.
+  iMod (heap_bij_shared_alloc with "[$]") as "[? #$]"; [done|]. iModIntro.
   iSplit. 2: { iPureIntro. by rewrite Hl0 offset_loc_0. } iFrame.
   iApply big_sepM_insert; [done|]. iFrame. iRight. by iFrame.
 Qed.
 
-Lemma heap_in_inj_free hi hs li ls rem:
+Lemma heap_in_bij_free hi hs li ls rem:
   ls.1 ∉ rem →
   ls.2 = 0%Z →
-  heap_inj_inv_i hi -∗
-  heap_inj_inv_s hs -∗
-  loc_in_inj li ls -∗
-  heap_in_inj rem ==∗
-  heap_in_inj rem ∗
-  heap_inj_inv_i (heap_free hi li) ∗
-  heap_inj_inv_s (heap_free hs ls).
+  heap_bij_inv_i hi -∗
+  heap_bij_inv_s hs -∗
+  loc_in_bij li ls -∗
+  heap_in_bij rem ==∗
+  heap_in_bij rem ∗
+  heap_bij_inv_i (heap_free hi li) ∗
+  heap_bij_inv_s (heap_free hs ls).
 Proof.
-  iIntros (? Hls2) "Hinvi Hinvs [% [-> #Hl]] Hinj".
+  iIntros (? Hls2) "Hinvi Hinvs [% [-> #Hl]] Hbij".
   rewrite Hls2 offset_loc_0.
-  iDestruct (heap_in_inj_borrow with "[$] [$]") as (???) "[? [? [??]]]"; [done|].
+  iDestruct (heap_in_bij_borrow with "[$] [$]") as (???) "[? [? [??]]]"; [done|].
   iDestruct (heapUR_lookup_block with "Hinvi [$]") as %<-.
   iDestruct (heapUR_lookup_block with "Hinvs [$]") as %<-.
   iMod (heapUR_free with "[$] [$]") as "[$ ?]".
   iMod (heapUR_free with "[$] [$]") as "[$ ?]". iModIntro.
-  iApply (heap_in_inj_return0 with "[$] [$] [$] [$]"); [done|].
+  iApply (heap_in_bij_return0 with "[$] [$] [$] [$]"); [done|].
   by iApply big_sepM2_empty.
 Qed.
 
-(** * heap_inj_inv *)
-Definition heap_inj_inv (hi hs : heap_state) (rem : list prov) : uPred heap_injUR :=
-  heap_inj_inv_i hi ∗
-  heap_inj_inv_s hs ∗
-  heap_in_inj rem ∗
-  heap_inj_statics (h_static_provs hi) ∗
-  heap_inj_statics (h_static_provs hs).
+(** * heap_bij_inv *)
+Definition heap_bij_inv (hi hs : heap_state) (rem : list prov) : uPred heap_bijUR :=
+  heap_bij_inv_i hi ∗
+  heap_bij_inv_s hs ∗
+  heap_in_bij rem ∗
+  heap_bij_statics (h_static_provs hi) ∗
+  heap_bij_statics (h_static_provs hs).
 
 
-Lemma heap_inj_inv_range hi hs l1 l2 z rem:
+Lemma heap_bij_inv_range hi hs l1 l2 z rem:
   l2.2 = 0%Z →
   heap_range hs l2 z →
   l2.1 ∉ rem →
-  heap_inj_inv hi hs rem -∗
-  loc_in_inj l1 l2 -∗
+  heap_bij_inv hi hs rem -∗
+  loc_in_bij l1 l2 -∗
   ⌜heap_range hi l1 z⌝.
 Proof.
   iIntros (???) "[Hinvi [Hinvs[?[??]]]]".
-  by iApply (heap_in_inj_range with "[$] [$] [$]").
+  by iApply (heap_in_bij_range with "[$] [$] [$]").
 Qed.
 
-Lemma heap_inj_inv_lookup hi hs li ls v rem:
+Lemma heap_bij_inv_lookup hi hs li ls v rem:
   h_heap hs !! ls = Some v →
   ls.1 ∉ rem →
-  heap_inj_inv hi hs rem -∗
-  loc_in_inj li ls -∗
-  ∃ v', ⌜h_heap hi !! li = Some v'⌝ ∗ val_in_inj v' v.
+  heap_bij_inv hi hs rem -∗
+  loc_in_bij li ls -∗
+  ∃ v', ⌜h_heap hi !! li = Some v'⌝ ∗ val_in_bij v' v.
 Proof.
   iIntros (??) "[Hinvi [Hinvs[?[??]]]]".
-  by iApply (heap_in_inj_lookup with "[$] [$] [$]").
+  by iApply (heap_in_bij_lookup with "[$] [$] [$]").
 Qed.
 
-Lemma heap_inj_inv_alive hi hs li ls rem:
+Lemma heap_bij_inv_alive hi hs li ls rem:
   heap_alive hs ls →
   ls.1 ∉ rem →
-  heap_inj_inv hi hs rem -∗
-  loc_in_inj li ls -∗
+  heap_bij_inv hi hs rem -∗
+  loc_in_bij li ls -∗
   ⌜heap_alive hi li⌝.
 Proof.
   iIntros ([??]?) "??".
-  iDestruct (heap_inj_inv_lookup with "[$] [$]") as (??) "?"; [done..|].
+  iDestruct (heap_bij_inv_lookup with "[$] [$]") as (??) "?"; [done..|].
   iPureIntro. by eexists _.
 Qed.
 
-Lemma heap_inj_inv_lookup_dom_i p hi hs d rem dq:
-  heap_inj_inv hi hs rem -∗
+Lemma heap_bij_inv_lookup_dom_i p hi hs d rem dq:
+  heap_bij_inv hi hs rem -∗
   p ⤚hi{dq} d -∗
   ⌜dom (h_block hi p) = d⌝.
 Proof.
@@ -511,8 +511,8 @@ Proof.
   by iApply (heapUR_lookup_dom with "Hinvi").
 Qed.
 
-Lemma heap_inj_inv_lookup_dom_s p hi hs d rem dq:
-  heap_inj_inv hi hs rem -∗
+Lemma heap_bij_inv_lookup_dom_s p hi hs d rem dq:
+  heap_bij_inv hi hs rem -∗
   p ⤚hs{dq} d -∗
   ⌜dom (h_block hs p) = d⌝.
 Proof.
@@ -520,8 +520,8 @@ Proof.
   by iApply (heapUR_lookup_dom with "Hinvs").
 Qed.
 
-Lemma heap_inj_inv_lookup_block_i p hi hs b rem dq:
-  heap_inj_inv hi hs rem -∗
+Lemma heap_bij_inv_lookup_block_i p hi hs b rem dq:
+  heap_bij_inv hi hs rem -∗
   p ↦∗hi{dq} b -∗
   ⌜h_block hi p = b⌝.
 Proof.
@@ -529,8 +529,8 @@ Proof.
   by iApply (heapUR_lookup_block with "Hinvi").
 Qed.
 
-Lemma heap_inj_inv_lookup_block_s p hi hs b rem dq:
-  heap_inj_inv hi hs rem -∗
+Lemma heap_bij_inv_lookup_block_s p hi hs b rem dq:
+  heap_bij_inv hi hs rem -∗
   p ↦∗hs{dq} b -∗
   ⌜h_block hs p = b⌝.
 Proof.
@@ -538,24 +538,24 @@ Proof.
   by iApply (heapUR_lookup_block with "Hinvs").
 Qed.
 
-Lemma heap_inj_inv_update hi hs li ls vi vs rem :
+Lemma heap_bij_inv_update hi hs li ls vi vs rem :
   ls.1 ∉ rem →
   heap_alive hs ls →
-  heap_inj_inv hi hs rem -∗
-  loc_in_inj li ls -∗
-  val_in_inj vi vs ==∗
-  heap_inj_inv (heap_update hi li vi) (heap_update hs ls vs) rem.
+  heap_bij_inv hi hs rem -∗
+  loc_in_bij li ls -∗
+  val_in_bij vi vs ==∗
+  heap_bij_inv (heap_update hi li vi) (heap_update hs ls vs) rem.
 Proof.
   iIntros (??) "(Hinvi&Hinvs&?&?&?) ? ?".
-  iMod (heap_in_inj_update with "[$] [$] [$] [$] [$]") as "[$ [$ $]]"; [done..|].
+  iMod (heap_in_bij_update with "[$] [$] [$] [$] [$]") as "[$ [$ $]]"; [done..|].
   iModIntro. rewrite !h_static_provs_heap_update. iFrame.
 Qed.
 
-Lemma heap_inj_inv_update_in_block_i hi hs li v rem b :
+Lemma heap_bij_inv_update_in_block_i hi hs li v rem b :
   heap_alive hi li →
-  heap_inj_inv hi hs rem -∗
+  heap_bij_inv hi hs rem -∗
   li.1 ↦∗hi b ==∗
-  heap_inj_inv (heap_update hi li v) hs rem ∗
+  heap_bij_inv (heap_update hi li v) hs rem ∗
   li.1 ↦∗hi (<[li.2 :=v]> b).
 Proof.
   iIntros (?) "(?&$&$&?&$) ?".
@@ -563,11 +563,11 @@ Proof.
   by rewrite h_static_provs_heap_update.
 Qed.
 
-Lemma heap_inj_inv_update_in_block_s hi hs ls vs rem b :
+Lemma heap_bij_inv_update_in_block_s hi hs ls vs rem b :
   heap_alive hs ls →
-  heap_inj_inv hi hs rem -∗
+  heap_bij_inv hi hs rem -∗
   ls.1 ↦∗hs b ==∗
-  heap_inj_inv hi (heap_update hs ls vs) rem ∗
+  heap_bij_inv hi (heap_update hs ls vs) rem ∗
   ls.1 ↦∗hs (<[ls.2:=vs]> b).
 Proof.
   iIntros (?) "($&Hinvs&$&$&?) ?".
@@ -575,102 +575,102 @@ Proof.
   by rewrite h_static_provs_heap_update.
 Qed.
 
-Lemma heap_inj_inv_alloc_i hi hs li n rem:
+Lemma heap_bij_inv_alloc_i hi hs li n rem:
   heap_is_fresh hi li →
-  heap_inj_inv hi hs rem ==∗
-  heap_inj_inv (heap_alloc hi li n) hs rem ∗
+  heap_bij_inv hi hs rem ==∗
+  heap_bij_inv (heap_alloc hi li n) hs rem ∗
   li.1 ↦∗hi (zero_block n).
 Proof.
   iIntros (Hf) "(?&$&$&?&$)". iMod (heapUR_alloc with "[$]") as "[$ $]"; [done|].
   rewrite h_static_provs_heap_alloc //. by destruct Hf as [?[??]].
 Qed.
 
-Lemma heap_inj_inv_alloc_s hi hs ls n rem:
+Lemma heap_bij_inv_alloc_s hi hs ls n rem:
   heap_is_fresh hs ls →
-  heap_inj_inv hi hs rem ==∗
-  heap_inj_inv hi (heap_alloc hs ls n) rem ∗
+  heap_bij_inv hi hs rem ==∗
+  heap_bij_inv hi (heap_alloc hs ls n) rem ∗
   ls.1 ↦∗hs (zero_block n).
 Proof.
   iIntros (Hf) "($&?&$&$&?)". iMod (heapUR_alloc with "[$]") as "[$ $]"; [done|].
   rewrite h_static_provs_heap_alloc //. by destruct Hf as [?[??]].
 Qed.
 
-Lemma heap_inj_inv_alloc hi hs li ls n rem:
+Lemma heap_bij_inv_alloc hi hs li ls n rem:
   heap_is_fresh hi li →
   heap_is_fresh hs ls →
   ls.1 ∉ rem →
-  heap_inj_inv hi hs rem ==∗
-  heap_inj_inv (heap_alloc hi li n) (heap_alloc hs ls n) rem ∗
-  loc_in_inj li ls.
+  heap_bij_inv hi hs rem ==∗
+  heap_bij_inv (heap_alloc hi li n) (heap_alloc hs ls n) rem ∗
+  loc_in_bij li ls.
 Proof.
   iIntros (Hi Hs ?) "?". have Hli0 : li.2 = 0 by destruct Hi as [?[??]].
-  iMod (heap_inj_inv_alloc_i with "[$]") as "[? ?]"; [done|].
-  iMod (heap_inj_inv_alloc_s with "[$]") as "[Hinv ?]"; [done|].
+  iMod (heap_bij_inv_alloc_i with "[$]") as "[? ?]"; [done|].
+  iMod (heap_bij_inv_alloc_s with "[$]") as "[Hinv ?]"; [done|].
   iDestruct "Hinv" as "($ & $ &?& $ & $)".
-  iMod (heap_in_inj_share with "[$] [$] [$] []") as "[$ $]"; [done..| | |done].
+  iMod (heap_in_bij_share with "[$] [$] [$] []") as "[$ $]"; [done..| | |done].
   { destruct Hs. naive_solver. }
   iApply big_sepM_sepM2_diag. iApply big_sepM_intro.
   iIntros "!>" (??[-> ?]%zero_block_lookup_Some). done.
 Qed.
 
-Lemma heap_inj_inv_alloc_list hi hs hi' hs' xs lsi lss:
+Lemma heap_bij_inv_alloc_list hi hs hi' hs' xs lsi lss:
   heap_alloc_list xs lsi hi hi' →
   heap_alloc_list xs lss hs hs' →
-  heap_inj_inv hi hs [] ==∗
-  heap_inj_inv hi' hs' [] ∗
-  ([∗ list] li;ls∈lsi;lss, loc_in_inj li ls).
+  heap_bij_inv hi hs [] ==∗
+  heap_bij_inv hi' hs' [] ∗
+  ([∗ list] li;ls∈lsi;lss, loc_in_bij li ls).
 Proof.
   iIntros (Hi Hs) "Hinv".
   iInduction xs as [] "IH" forall (lsi lss hi hi' hs hs' Hi Hs); simplify_eq/=; destruct!/=.
   { by iFrame. }
-  iMod (heap_inj_inv_alloc with "Hinv") as "[Hinv $]"; [done..|set_solver|].
+  iMod (heap_bij_inv_alloc with "Hinv") as "[Hinv $]"; [done..|set_solver|].
   by iApply "IH".
 Qed.
 
-Lemma heap_inj_inv_free_i l hi hs b rem:
-  heap_inj_inv hi hs rem -∗
+Lemma heap_bij_inv_free_i l hi hs b rem:
+  heap_bij_inv hi hs rem -∗
   l.1 ↦∗hi b ==∗
-  heap_inj_inv (heap_free hi l) hs rem ∗ l.1 ↦∗hi ∅.
+  heap_bij_inv (heap_free hi l) hs rem ∗ l.1 ↦∗hi ∅.
 Proof.
   iIntros "[Hinvi [Hinvs[?[??]]]] ?".
   iMod (heapUR_free with "Hinvi [$]") as "[$ $]". iFrame.
   by rewrite h_static_provs_heap_free.
 Qed.
 
-Lemma heap_inj_inv_free_s l hi hs b rem:
-  heap_inj_inv hi hs rem -∗
+Lemma heap_bij_inv_free_s l hi hs b rem:
+  heap_bij_inv hi hs rem -∗
   l.1 ↦∗hs b ==∗
-  heap_inj_inv hi (heap_free hs l) rem ∗ l.1 ↦∗hs ∅.
+  heap_bij_inv hi (heap_free hs l) rem ∗ l.1 ↦∗hs ∅.
 Proof.
   iIntros "[Hinvi [Hinvs[?[??]]]] ?".
   iMod (heapUR_free with "Hinvs [$]") as "[$ $]". iFrame.
   by rewrite h_static_provs_heap_free.
 Qed.
 
-Lemma heap_inj_inv_free hi hs li ls rem n:
+Lemma heap_bij_inv_free hi hs li ls rem n:
   ls.1 ∉ rem →
   li.2 = 0%Z →
   ls.2 = 0%Z →
   heap_range hs ls n →
-  heap_inj_inv hi hs rem -∗
-  loc_in_inj li ls ==∗
-  heap_inj_inv (heap_free hi li) (heap_free hs ls) rem.
+  heap_bij_inv hi hs rem -∗
+  loc_in_bij li ls ==∗
+  heap_bij_inv (heap_free hi li) (heap_free hs ls) rem.
 Proof.
   iIntros (? ?? ?) "[Hinvi [Hinvs [? [? ?]]]] Hl".
-  iMod (heap_in_inj_free with "[$] [$] [$] [$]") as "[$ [$ $]]"; [done..|].
+  iMod (heap_in_bij_free with "[$] [$] [$] [$]") as "[$ [$ $]]"; [done..|].
   rewrite !h_static_provs_heap_free. by iFrame.
 Qed.
 
-Lemma heap_inj_inv_free_list hi hs hs' lis lss lis' lss' xsi xss hi0 hi0' hs0 hs0':
+Lemma heap_bij_inv_free_list hi hs hs' lis lss lis' lss' xsi xss hi0 hi0' hs0 hs0':
   heap_free_list lss hs hs' →
   lis.*2 = lss.*2 →
   lis' = lis.*1 →
   lss' = lss.*1 →
   heap_alloc_list xsi lis' hi0 hi0' →
   heap_alloc_list xss lss' hs0 hs0' →
-  heap_inj_inv hi hs [] -∗
-  ([∗ list] li;ls∈lis';lss', loc_in_inj li ls) ==∗
-  ∃ hi', ⌜heap_free_list lis hi hi'⌝ ∗ heap_inj_inv hi' hs' [].
+  heap_bij_inv hi hs [] -∗
+  ([∗ list] li;ls∈lis';lss', loc_in_bij li ls) ==∗
+  ∃ hi', ⌜heap_free_list lis hi hi'⌝ ∗ heap_bij_inv hi' hs' [].
 Proof.
   iIntros (Hf Hl2 -> -> Hai Has) "Hinv Hls".
   iInduction lss as [|[ls ?] lss] "IH" forall (hi hs hs' lis xsi xss hi0 hs0 Hf Hl2 Hai Has);
@@ -680,58 +680,58 @@ Proof.
   iDestruct "Hls" as "[Hl Hls]".
   iAssert ⌜heap_range hi l0 z⌝%I as %?. {
     iDestruct "Hinv" as "(?&?&?&?)".
-    iApply (heap_in_inj_range with "[$] [$] [$] [$]"); [done..| set_solver].
+    iApply (heap_in_bij_range with "[$] [$] [$] [$]"); [done..| set_solver].
   }
-  iMod (heap_inj_inv_free with "[$] [$]") as "[??]"; [set_solver|done..|].
+  iMod (heap_bij_inv_free with "[$] [$]") as "[??]"; [set_solver|done..|].
   iMod ("IH" with "[//] [//] [//] [//] [$] [$]") as (??) "?". iModIntro. by iFrame.
 Qed.
 
 (* specialized to the same provenance and heap on both sides for now
 since this suffices for statics *)
-Lemma heap_inj_inv_share hi hs p h:
-  heap_inj_inv hi hs [] -∗
+Lemma heap_bij_inv_share hi hs p h:
+  heap_bij_inv hi hs [] -∗
   p ↦∗hi h -∗
   p ↦∗hs h -∗
-  ([∗ map] v∈h, val_in_inj v v) ==∗
-  heap_inj_inv hi hs [] ∗ loc_in_inj (p, 0%Z) (p, 0%Z).
+  ([∗ map] v∈h, val_in_bij v v) ==∗
+  heap_bij_inv hi hs [] ∗ loc_in_bij (p, 0%Z) (p, 0%Z).
 Proof.
   iIntros "($&$&?&$&$) Hi Hs #Hv".
-  iMod (heap_in_inj_share (p, 0%Z) (p, 0%Z) with "[$] [$] [$] []") as "[$ $]"; [set_solver|done|done| |done].
+  iMod (heap_in_bij_share (p, 0%Z) (p, 0%Z) with "[$] [$] [$] []") as "[$ $]"; [set_solver|done|done| |done].
   by iApply (big_sepM_sepM2_diag).
 Qed.
 
-Lemma heap_inj_inv_share_big hi hs m:
-  heap_inj_inv hi hs [] -∗
+Lemma heap_bij_inv_share_big hi hs m:
+  heap_bij_inv hi hs [] -∗
   ([∗ map] p↦h∈m, p ↦∗hi h) -∗
   ([∗ map] p↦h∈m, p ↦∗hs h) -∗
-  ([∗ map] p↦h∈m, [∗ map] v∈h, val_in_inj v v) ==∗
-  heap_inj_inv hi hs [] ∗ ([∗ map] p↦h∈m, loc_in_inj (p, 0%Z) (p, 0%Z)).
+  ([∗ map] p↦h∈m, [∗ map] v∈h, val_in_bij v v) ==∗
+  heap_bij_inv hi hs [] ∗ ([∗ map] p↦h∈m, loc_in_bij (p, 0%Z) (p, 0%Z)).
 Proof.
   iIntros "Hinv Hi Hs Hv".
   iInduction m as [|???] "IH" using map_ind. { iModIntro. by iFrame. }
   rewrite !big_sepM_insert //.
-  iDestruct!. iMod (heap_inj_inv_share with "[$] [$] [$] [$]") as "[? $]".
+  iDestruct!. iMod (heap_bij_inv_share with "[$] [$] [$] [$]") as "[? $]".
   by iApply ("IH" with "[$] [$] [$] [$]").
 Qed.
 
-Definition rec_heap_inj_init (h0 : gmap prov (gmap Z val)) : uPred heap_injUR :=
+Definition rec_heap_bij_init (h0 : gmap prov (gmap Z val)) : uPred heap_bijUR :=
   (([∗ map]p↦v∈h0, p ↦∗hi v) ∗ ([∗ map]p↦v∈h0, p ↦∗hs v)).
 
-Lemma rec_heap_inj_init_union h1 h2:
+Lemma rec_heap_bij_init_union h1 h2:
   h1 ##ₘ h2 →
-  rec_heap_inj_init (h1 ∪ h2) ⊣⊢ rec_heap_inj_init h1 ∗ rec_heap_inj_init h2.
+  rec_heap_bij_init (h1 ∪ h2) ⊣⊢ rec_heap_bij_init h1 ∗ rec_heap_bij_init h2.
 Proof.
-  move => Hdisj. rewrite /rec_heap_inj_init.
+  move => Hdisj. rewrite /rec_heap_bij_init.
   rewrite !big_sepM_union //. iSplit; iIntros!; iFrame.
 Qed.
 
-Lemma heap_inj_inv_share_init hi hs f statics :
-  heap_inj_inv hi hs [] -∗
-  rec_heap_inj_init (fd_init_heap f statics) ==∗
-  ([∗ list] l ∈ static_locs f statics, loc_in_inj l l) ∗ heap_inj_inv hi hs [].
+Lemma heap_bij_inv_share_init hi hs f statics :
+  heap_bij_inv hi hs [] -∗
+  rec_heap_bij_init (fd_init_heap f statics) ==∗
+  ([∗ list] l ∈ static_locs f statics, loc_in_bij l l) ∗ heap_bij_inv hi hs [].
 Proof.
   iIntros "Hinv [Hi Hs]".
-  iMod (heap_inj_inv_share_big with "Hinv Hi Hs []") as "[$ ?]". {
+  iMod (heap_bij_inv_share_big with "Hinv Hi Hs []") as "[$ ?]". {
     iApply big_sepM_intro. iIntros "!>" (??[?[?[?[??]]]]%fd_init_heap_lookup_Some).
     simplify_eq. iApply big_sepM_intro.
     iIntros "!>" (??[??]%zero_block_lookup_Some); by simplify_eq/=.
@@ -747,26 +747,26 @@ Proof.
   case_match eqn: Heq => //. apply lookup_ge_None in Heq. lia.
 Qed.
 
-Lemma heap_inj_inv_share_inits hi hs fns :
-  heap_inj_inv hi hs [] -∗
-  rec_heap_inj_init (fds_init_heap fns) ==∗
-  ([∗ map] f↦fn∈fns, [∗ list] l ∈ static_locs f fn, loc_in_inj l l) ∗ heap_inj_inv hi hs [].
+Lemma heap_bij_inv_share_inits hi hs fns :
+  heap_bij_inv hi hs [] -∗
+  rec_heap_bij_init (fds_init_heap fns) ==∗
+  ([∗ map] f↦fn∈fns, [∗ list] l ∈ static_locs f fn, loc_in_bij l l) ∗ heap_bij_inv hi hs [].
 Proof.
   iIntros "Hinv Hinit".
   iInduction fns as [|f fn fns Hf] "IH" using map_ind forall (hi hs).
   { iModIntro. iFrame. done. }
-  rewrite fds_init_heap_insert // rec_heap_inj_init_union.
+  rewrite fds_init_heap_insert // rec_heap_bij_init_union.
   2: by apply fds_init_heap_map_disjoint.
   iDestruct "Hinit" as "[? Hinit2]".
   iMod ("IH" with "Hinv Hinit2") as "[? Hinv]".
-  iMod (heap_inj_inv_share_init with "[$] [$]") as "[??]".
+  iMod (heap_bij_inv_share_init with "[$] [$]") as "[??]".
   iModIntro. rewrite big_sepM_insert //. iFrame.
 Qed.
 
 
-Lemma heap_inj_init ps :
-  satisfiable (heap_inj_shared_auth ∅ ∗ heap_inj_statics ps
-                 ∗ heap_inj_inv_i ∅ ∗ heap_inj_inv_s ∅).
+Lemma heap_bij_init ps :
+  satisfiable (heap_bij_shared_auth ∅ ∗ heap_bij_statics ps
+                 ∗ heap_bij_inv_i ∅ ∗ heap_bij_inv_s ∅).
 Proof.
   apply: (satisfiable_init (Some (to_agree ps),
               (gmap_view_auth (DfracOwn 1) ∅,
@@ -777,129 +777,129 @@ Proof.
   rewrite (pair_split (Some _)) uPred.ownM_op.
   rewrite (pair_split (gmap_view_auth _ _)) pair_op_2 uPred.ownM_op.
   rewrite (pair_split (heapUR_init)) !pair_op_2 uPred.ownM_op.
-  iIntros!. rewrite -!heapUR_init_own /heap_inj_shared_auth big_sepM_empty. by iFrame.
+  iIntros!. rewrite -!heapUR_init_own /heap_bij_shared_auth big_sepM_empty. by iFrame.
 Qed.
 
-Lemma heap_inj_inv_init bs :
-  satisfiable (heap_inj_inv (heap_from_blocks bs) (heap_from_blocks bs) [] ∗ rec_heap_inj_init bs).
+Lemma heap_bij_inv_init bs :
+  satisfiable (heap_bij_inv (heap_from_blocks bs) (heap_from_blocks bs) [] ∗ rec_heap_bij_init bs).
 Proof.
-  apply: satisfiable_bmono; [apply heap_inj_init|].
+  apply: satisfiable_bmono; [apply heap_bij_init|].
   iIntros "(? & #? & Hinvi & Hinvs)".
   iMod (heapUR_alloc_blocks with "Hinvi") as "[Hinvi $]"; [set_solver|].
   iMod (heapUR_alloc_blocks with "Hinvs") as "[Hinvs $]"; [set_solver|].
   iModIntro. rewrite right_id. iFrame "Hinvi Hinvs #".
-  by iApply heap_in_inj_init.
+  by iApply heap_in_bij_init.
 Qed.
 
-(** * Definition of [rec_heap_inj] *)
-Definition rec_heap_inj_pre (e : rec_event) (s : unit) : prepost (rec_event * unit) heap_injUR :=
+(** * Definition of [rec_heap_bij] *)
+Definition rec_heap_bij_pre (e : rec_event) (s : unit) : prepost (rec_event * unit) heap_bijUR :=
   let vsi := vals_of_event e.2 in
   let hi := heap_of_event e.2 in
   pp_quant $ λ vss,
   pp_quant $ λ hs,
-  pp_star (heap_inj_inv hi hs [] ∗ [∗ list] v1;v2∈vsi;vss, val_in_inj v1 v2) $
+  pp_star (heap_bij_inv hi hs [] ∗ [∗ list] v1;v2∈vsi;vss, val_in_bij v1 v2) $
   pp_end ((e.1, event_set_vals_heap e.2 vss hs), tt).
 
-Definition rec_heap_inj_post (e : rec_event) (s : unit) : prepost (rec_event * unit) heap_injUR :=
+Definition rec_heap_bij_post (e : rec_event) (s : unit) : prepost (rec_event * unit) heap_bijUR :=
   let vss := vals_of_event e.2 in
   let hs := heap_of_event e.2 in
   pp_quant $ λ vsi,
   pp_quant $ λ hi,
-  pp_star (heap_inj_inv hi hs [] ∗ [∗ list] v1;v2∈vsi;vss, val_in_inj v1 v2) $
+  pp_star (heap_bij_inv hi hs [] ∗ [∗ list] v1;v2∈vsi;vss, val_in_bij v1 v2) $
   pp_end ((e.1, event_set_vals_heap e.2 vsi hi), tt).
 
-Definition rec_heap_inj_trans (m : mod_trans rec_event) : mod_trans rec_event :=
-  prepost_trans rec_heap_inj_pre rec_heap_inj_post m.
+Definition rec_heap_bij_trans (m : mod_trans rec_event) : mod_trans rec_event :=
+  prepost_trans rec_heap_bij_pre rec_heap_bij_post m.
 
-Definition rec_heap_inj (h0 : gmap prov (gmap Z val)) (m : module rec_event) : module rec_event :=
-  Mod (rec_heap_inj_trans m.(m_trans)) (SMFilter, m.(m_init), (PPOutside, tt,
-   uPred_shrink (rec_heap_inj_init h0))).
+Definition rec_heap_bij (h0 : gmap prov (gmap Z val)) (m : module rec_event) : module rec_event :=
+  Mod (rec_heap_bij_trans m.(m_trans)) (SMFilter, m.(m_init), (PPOutside, tt,
+   uPred_shrink (rec_heap_bij_init h0))).
 
-Lemma rec_heap_inj_trefines m m' h0 `{!VisNoAng m.(m_trans)}:
+Lemma rec_heap_bij_trefines m m' h0 `{!VisNoAng m.(m_trans)}:
   trefines m m' →
-  trefines (rec_heap_inj h0 m) (rec_heap_inj h0 m').
+  trefines (rec_heap_bij h0 m) (rec_heap_bij h0 m').
 Proof. move => ?. by apply: prepost_mod_trefines. Qed.
 
-(** ** rec_heap_inj_N *)
-Definition rec_heap_inj_N n h0 (m: module rec_event) : module rec_event :=
-  Nat.iter n (rec_heap_inj h0) m.
+(** ** rec_heap_bij_N *)
+Definition rec_heap_bij_N n h0 (m: module rec_event) : module rec_event :=
+  Nat.iter n (rec_heap_bij h0) m.
 
-Global Instance rec_heap_inj_N_vis_no_all n m h0 `{!VisNoAng m.(m_trans)} :
-  VisNoAng (rec_heap_inj_N n h0 m).(m_trans).
+Global Instance rec_heap_bij_N_vis_no_all n m h0 `{!VisNoAng m.(m_trans)} :
+  VisNoAng (rec_heap_bij_N n h0 m).(m_trans).
 Proof. elim: n => //= ??. apply _. Qed.
 
-(** * Proof techniques for [rec_heap_inj] *)
-Definition rec_heap_inj_call (n : ordinal) (fns1 fns2 : gmap string fndef) INV :=
+(** * Proof techniques for [rec_heap_bij] *)
+Definition rec_heap_bij_call (n : ordinal) (fns1 fns2 : gmap string fndef) INV :=
   (∀ n' f es1' es2' K1' K2' es1 es2 vs1' vs2' h1' h2' b r rf',
       RecExprFill es1' K1' (Call (Val (ValFn f)) es1) →
       RecExprFill es2' K2' (Call (Val (ValFn f)) es2) →
       n' ⊆ n →
       Forall2 (λ e v, e = Val v) es1 vs1' →
       Forall2 (λ e v, e = Val v) es2 vs2' →
-      satisfiable (heap_inj_inv h1' h2' [] ∗ ([∗ list] v1;v2∈vs1';vs2', val_in_inj v1 v2) ∗ INV ∗ r ∗ rf') →
+      satisfiable (heap_bij_inv h1' h2' [] ∗ ([∗ list] v1;v2∈vs1';vs2', val_in_bij v1 v2) ∗ INV ∗ r ∗ rf') →
       (∀ v1'' v2'' h1'' h2'' rf'',
-        satisfiable (heap_inj_inv h1'' h2'' [] ∗ val_in_inj v1'' v2'' ∗ INV ∗ r ∗ rf'') →
+        satisfiable (heap_bij_inv h1'' h2'' [] ∗ val_in_bij v1'' v2'' ∗ INV ∗ r ∗ rf'') →
         Rec (expr_fill K1' (Val v1'')) h1'' fns1
-            ⪯{rec_trans, rec_heap_inj_trans rec_trans, n', true}
+            ⪯{rec_trans, rec_heap_bij_trans rec_trans, n', true}
         (SMProg, Rec (expr_fill K2' (Val v2'')) h2'' fns2, (PPInside, tt, uPred_shrink rf''))) →
       Rec es1' h1' fns1
-          ⪯{rec_trans, rec_heap_inj_trans rec_trans, n', b}
+          ⪯{rec_trans, rec_heap_bij_trans rec_trans, n', b}
       (SMProg, Rec es2' h2' fns2, (PPInside, tt, uPred_shrink rf'))).
 
-Definition rec_heap_inj_return n fns1 fns2 Ki Ks r INV :=
+Definition rec_heap_bij_return n fns1 fns2 Ki Ks r INV :=
   (∀ n' v1 v2 h1' h2' rf' b,
       n' ⊆ n →
-      satisfiable (heap_inj_inv h1' h2' [] ∗ val_in_inj v1 v2 ∗ INV ∗ r ∗ rf') →
+      satisfiable (heap_bij_inv h1' h2' [] ∗ val_in_bij v1 v2 ∗ INV ∗ r ∗ rf') →
       Rec (expr_fill Ki (Val v1)) h1' fns1
-        ⪯{rec_trans, rec_heap_inj_trans rec_trans, n', b}
+        ⪯{rec_trans, rec_heap_bij_trans rec_trans, n', b}
       (SMProg, Rec (expr_fill Ks (Val v2)) h2' fns2, (PPInside, (), uPred_shrink rf'))).
 
-Lemma rec_heap_inj_call_mono n n' fns1 fns2 INV :
-  rec_heap_inj_call n fns1 fns2 INV →
+Lemma rec_heap_bij_call_mono n n' fns1 fns2 INV :
+  rec_heap_bij_call n fns1 fns2 INV →
   n' ⊆ n →
-  rec_heap_inj_call n' fns1 fns2 INV .
+  rec_heap_bij_call n' fns1 fns2 INV .
 Proof.
   intros Hprf ???????????????????????.
   eapply Hprf; eauto. by etrans.
 Qed.
 
-Lemma rec_heap_inj_return_mono n n' fns1 fns2 K1 K2 r INV:
-  rec_heap_inj_return n fns1 fns2 K1 K2 r INV →
+Lemma rec_heap_bij_return_mono n n' fns1 fns2 K1 K2 r INV:
+  rec_heap_bij_return n fns1 fns2 K1 K2 r INV →
   n' ⊆ n →
-  rec_heap_inj_return n' fns1 fns2 K1 K2 r INV.
+  rec_heap_bij_return n' fns1 fns2 K1 K2 r INV.
 Proof.
   intros Hprf ??????????.
   eapply Hprf; eauto. by etrans.
 Qed.
 
-Lemma rec_heap_inj_proof INV fns1 fns2 h0 :
+Lemma rec_heap_bij_proof INV fns1 fns2 h0 :
   dom fns1 = dom fns2 →
   (∀ f fn1, fns1 !! f = Some fn1 → ∃ fn2, fns2 !! f = Some fn2
                                           ∧ length (fd_args fn1) = length (fd_args fn2)
                                           ∧ fd_static_vars fn1 = fd_static_vars fn2) →
-  (∀ hi hs, rec_heap_inj_init h0 -∗ heap_inj_inv hi hs [] ==∗ INV ∗ heap_inj_inv hi hs []) →
+  (∀ hi hs, rec_heap_bij_init h0 -∗ heap_bij_inv hi hs [] ==∗ INV ∗ heap_bij_inv hi hs []) →
   (∀ n K1 K2 f fn1 fn2 vs1 vs2 h1 h2 r rf,
       fns1 !! f = Some fn1 →
       fns2 !! f = Some fn2 →
       length vs1 = length (fd_args fn1) →
       length vs2 = length (fd_args fn2) →
-      satisfiable (heap_inj_inv h1 h2 [] ∗ ([∗ list] v1;v2∈vs1;vs2, val_in_inj v1 v2) ∗ INV ∗ r ∗ rf) →
+      satisfiable (heap_bij_inv h1 h2 [] ∗ ([∗ list] v1;v2∈vs1;vs2, val_in_bij v1 v2) ∗ INV ∗ r ∗ rf) →
 
-      rec_heap_inj_call n fns1 fns2 INV →
-      rec_heap_inj_return n fns1 fns2 K1 K2 r INV →
+      rec_heap_bij_call n fns1 fns2 INV →
+      rec_heap_bij_return n fns1 fns2 K1 K2 r INV →
 
       Rec (expr_fill K1 (AllocA fn1.(fd_vars) $ subst_static f (fd_static_vars fn1) $ subst_l fn1.(fd_args) vs1 (fd_body fn1))) h1 fns1
-          ⪯{rec_trans, rec_heap_inj_trans rec_trans, n, false}
+          ⪯{rec_trans, rec_heap_bij_trans rec_trans, n, false}
       (SMProg, Rec (expr_fill K2 (AllocA fn2.(fd_vars) $ subst_static f (fd_static_vars fn2) $ subst_l fn2.(fd_args) vs2 (fd_body fn2))) h2 fns2, (PPInside, tt, uPred_shrink rf))) →
-  trefines (rec_mod fns1) (rec_heap_inj h0 (rec_mod fns2)).
+  trefines (rec_mod fns1) (rec_heap_bij h0 (rec_mod fns2)).
 Proof.
   move => Hdom Hlen Hinit Hf.
-  rewrite (lock (dom _)) in Hdom. unfold rec_heap_inj.
+  rewrite (lock (dom _)) in Hdom. unfold rec_heap_bij.
   etrans. 2: {
     apply (mod_prepost_impl_prop _ _ _ _ INV); [apply _| ] => /=.
     iIntros (???) "? [[? ?] $]".
     iMod (Hinit with "[$] [$]") as "[$ $]". by iFrame. }
-  pose (R := λ (b : bool) (s1 s2 : (unit * uPred heap_injUR)), (if b then s1.2 ≡ s2.2 else True) ∧ (s2.2 ⊢ INV ∗ (INV -∗ s2.2))).
+  pose (R := λ (b : bool) (s1 s2 : (unit * uPred heap_bijUR)), (if b then s1.2 ≡ s2.2 else True) ∧ (s2.2 ⊢ INV ∗ (INV -∗ s2.2))).
   apply: (rec_prepost_proof R); unfold R; [| | naive_solver.. |].
   { destruct b.
     - move => ??? [-> ?] //.
@@ -922,11 +922,11 @@ Proof.
        length vs1 = length (fd_args fn1) ∧
        σfs = SMProg ∧
        t1 = PPInside ∧
-       satisfiable (heap_inj_inv h1 h2 []
-            ∗ ([∗ list] v1;v2∈vs1;vs2, val_in_inj v1 v2)
+       satisfiable (heap_bij_inv h1 h2 []
+            ∗ ([∗ list] v1;v2∈vs1;vs2, val_in_bij v1 v2)
             ∗ INV
             ∗ r ∗ rrf') ∧
-       rec_heap_inj_return n' fns1 fns2 K1 K2 r INV). }
+       rec_heap_bij_return n' fns1 fns2 K1 K2 r INV). }
   { move => /= ??. split! => //; [lia|..]. {
       iSatMono. iFrame. iStopProof.
       etrans; [apply Hstat|]. iIntros!. iFrame. iAccu. } iSatClear.
@@ -957,13 +957,13 @@ Proof.
       iDestruct (big_sepL2_cons_inv_l with "[$]") as (???) "[??]". by simplify_eq.
 Qed.
 
-(** * Properties of [rec_heap_inj] *)
+(** * Properties of [rec_heap_bij] *)
 (** ** Horizontal compositionality *)
-Lemma rec_heap_inj_combine fns1 fns2 m1 m2 h01 h02 h0 `{!VisNoAng m1.(m_trans)} `{!VisNoAng m2.(m_trans)}:
+Lemma rec_heap_bij_combine fns1 fns2 m1 m2 h01 h02 h0 `{!VisNoAng m1.(m_trans)} `{!VisNoAng m2.(m_trans)}:
   h01 ##ₘ h02 →
   h0 = h01 ∪ h02 →
-  trefines (rec_link fns1 fns2 (rec_heap_inj h01 m1) (rec_heap_inj h02 m2))
-           (rec_heap_inj h0 (rec_link fns1 fns2 m1 m2)).
+  trefines (rec_link fns1 fns2 (rec_heap_bij h01 m1) (rec_heap_bij h02 m2))
+           (rec_heap_bij h0 (rec_link fns1 fns2 m1 m2)).
 Proof.
   move => Hdisj ->.
   unshelve apply: prepost_link. { exact
@@ -976,7 +976,7 @@ Proof.
         end
       ). }
   { move => ?? [] /=*; naive_solver. }
-  { split!. rewrite /rec_heap_inj_init !big_sepM_union //. iSplit; iIntros!; iFrame. }
+  { split!. rewrite /rec_heap_bij_init !big_sepM_union //. iSplit; iIntros!; iFrame. }
   all: move => [] [] [] P1 P2 P ics1 ics2.
   - move => e ics' e' /= ? ? *; destruct!/=.
     setoid_subst.
@@ -1013,17 +1013,17 @@ Proof.
 Qed.
 
 (** ** Reflexivity *)
-Lemma rec_heap_inj_sim_call_bind args vs' ws' es ei Ks Ki vss vsi vfi vfs n b hi hs fns1 fns2 rf r INV
+Lemma rec_heap_bij_sim_call_bind args vs' ws' es ei Ks Ki vss vsi vfi vfs n b hi hs fns1 fns2 rf r INV
   `{Hfill2: !RecExprFill ei Ki (Call (Val vfi) ((Val <$> vs') ++ (subst_map vsi <$> args)))}
   `{Hfill1: !RecExprFill es Ks (Call (Val vfs) ((Val <$> ws') ++ (subst_map vss <$> args)))}:
-    satisfiable (heap_inj_inv hi hs [] ∗ ([∗ map] vi;vs ∈ vsi; vss, val_in_inj vi vs) ∗ ([∗ list] v; w ∈ vs'; ws', val_in_inj v w) ∗ val_in_inj vfi vfs ∗ INV ∗ r ∗ rf) →
+    satisfiable (heap_bij_inv hi hs [] ∗ ([∗ map] vi;vs ∈ vsi; vss, val_in_bij vi vs) ∗ ([∗ list] v; w ∈ vs'; ws', val_in_bij v w) ∗ val_in_bij vfi vfs ∗ INV ∗ r ∗ rf) →
     dom vss ⊆ dom vsi →
-    rec_heap_inj_call n fns1 fns2 INV →
+    rec_heap_bij_call n fns1 fns2 INV →
     (∀ vs ws hi' hs' b' n' rf' f,
       n' ⊆ n →
-      satisfiable (heap_inj_inv hi' hs' [] ∗ ([∗ map] vi;vs ∈ vsi; vss, val_in_inj vi vs) ∗ ([∗ list] v; w ∈ vs' ++ vs; ws' ++ ws, val_in_inj v w) ∗ INV ∗ r ∗ rf') →
+      satisfiable (heap_bij_inv hi' hs' [] ∗ ([∗ map] vi;vs ∈ vsi; vss, val_in_bij vi vs) ∗ ([∗ list] v; w ∈ vs' ++ vs; ws' ++ ws, val_in_bij v w) ∗ INV ∗ r ∗ rf') →
       Rec (expr_fill Ki (Call (Val (ValFn f)) (Val <$> (vs' ++ vs)))) hi' fns1
-        ⪯{rec_trans, rec_heap_inj_trans rec_trans, n', b'}
+        ⪯{rec_trans, rec_heap_bij_trans rec_trans, n', b'}
       (SMProg, Rec (expr_fill Ks (Call (Val (ValFn f)) (Val <$> (ws' ++ ws)))) hs' fns2, (PPInside, (), uPred_shrink rf'))
     ) →
     Forall
@@ -1031,17 +1031,17 @@ Lemma rec_heap_inj_sim_call_bind args vs' ws' es ei Ks Ki vss vsi vfi vfs n b hi
        ∀ es ei hi hs n b Ki Ks r rf,
          RecExprFill es Ks (subst_map vss e)
          → RecExprFill ei Ki (subst_map vsi e)
-             → rec_heap_inj_call n fns1 fns2 INV
+             → rec_heap_bij_call n fns1 fns2 INV
                   → satisfiable
-                      (heap_inj_inv hi hs [] ∗
-                      ([∗ map] v1;v2 ∈ vsi;vss, val_in_inj v1 v2) ∗ INV ∗ r ∗
+                      (heap_bij_inv hi hs [] ∗
+                      ([∗ map] v1;v2 ∈ vsi;vss, val_in_bij v1 v2) ∗ INV ∗ r ∗
                       rf)
-                      → rec_heap_inj_return n fns1 fns2 Ki Ks r INV
+                      → rec_heap_bij_return n fns1 fns2 Ki Ks r INV
                      → Rec ei hi fns1 ⪯{rec_trans,
-                     rec_heap_inj_trans rec_trans, n, b}
+                     rec_heap_bij_trans rec_trans, n, b}
                      (SMProg, Rec es hs fns2, (PPInside, (), uPred_shrink rf))) args →
     Rec ei hi fns1
-      ⪯{rec_trans, rec_heap_inj_trans rec_trans, n, b}
+      ⪯{rec_trans, rec_heap_bij_trans rec_trans, n, b}
     (SMProg, Rec es hs fns2, (PPInside, (), uPred_shrink rf)).
 Proof.
   intros Hsat Hdom Hfuns Hcont Hargs; destruct Hfill1 as [->], Hfill2 as [->].
@@ -1055,7 +1055,7 @@ Proof.
   + eapply rec_expr_fill_expr_fill, (rec_expr_fill_expr_fill _ [CallCtx _ _ _]), rec_expr_fill_end.
   + eapply rec_expr_fill_expr_fill, (rec_expr_fill_expr_fill _ [CallCtx _ _ _]), rec_expr_fill_end.
   + done.
-  + iSatMono. iIntros "(Hinj & #Hvals & #Hvals' & Hf & Hs & r & rf)". iFrame.
+  + iSatMono. iIntros "(Hbij & #Hvals & #Hvals' & Hf & Hs & r & rf)". iFrame.
     iFrame "Hvals". iCombine "Hvals Hvals' Hf r" as "r". iExact "r".
   + simpl. iSatClear. intros n' v w h1' h2' rf' b' Hsub Hsat'. simpl.
     rewrite !cons_middle !app_assoc. change ([Val v]) with (Val <$> [v]).
@@ -1063,20 +1063,20 @@ Proof.
     specialize (IH (vs' ++ [v]) (ws' ++ [w]) n' b' h1' h2' rf').
     eapply IH; eauto.
     * iSatMono. iIntros!. by iFrame.
-    * by apply: rec_heap_inj_call_mono.
+    * by apply: rec_heap_bij_call_mono.
     * intros vs ws hi' hs' b'' n'' rf'' Hsub' Hsat. rewrite -!app_assoc.
       clear IH Hall Hsat'. eapply Hcont; first by etrans.
 Qed.
 
-Lemma rec_heap_inj_sim_refl_static INV vss vsi e es ei hi hs n b Ki Ks fns1 fns2 r rf
+Lemma rec_heap_bij_sim_refl_static INV vss vsi e es ei hi hs n b Ki Ks fns1 fns2 r rf
   `{Hfill1: !RecExprFill es Ks (subst_map vss e)}
   `{Hfill2: !RecExprFill ei Ki (subst_map vsi e)}:
   dom vss ⊆ dom vsi →
-  rec_heap_inj_call n fns1 fns2 INV →
-  rec_heap_inj_return n fns1 fns2 Ki Ks r INV →
+  rec_heap_bij_call n fns1 fns2 INV →
+  rec_heap_bij_return n fns1 fns2 Ki Ks r INV →
   is_static_expr false e →
-  satisfiable (heap_inj_inv hi hs [] ∗ ([∗ map] v1;v2 ∈ vsi; vss, val_in_inj v1 v2) ∗ INV ∗ r ∗ rf) →
-  Rec ei hi fns1 ⪯{rec_trans, rec_heap_inj_trans rec_trans, n, b} (SMProg, Rec es hs fns2, (PPInside, (), uPred_shrink rf)).
+  satisfiable (heap_bij_inv hi hs [] ∗ ([∗ map] v1;v2 ∈ vsi; vss, val_in_bij v1 v2) ∗ INV ∗ r ∗ rf) →
+  Rec ei hi fns1 ⪯{rec_trans, rec_heap_bij_trans rec_trans, n, b} (SMProg, Rec es hs fns2, (PPInside, (), uPred_shrink rf)).
 Proof.
   induction e as [x|v|e1 op e2 IH1 IH2|e IH|e1 e2 IH1 IH2|e e1 e2 IH IH1 IH2| x e1 e2 IH1 IH2| f args IH| | | |] in vss, vsi, hi, hs, n, b, Ks, Ki, es, ei, Hfill1, Hfill2, r, rf |-*;
     intros Hsub Hcall Hcont Hstatic Hsat;
@@ -1097,11 +1097,11 @@ Proof.
     iSatClear. intros n' vi vs hi' hs' rf' b' Hn' Hsat; simpl.
     apply: IH2; simpl; eauto; last first.
     { iSatMono. iIntros "($ & #Hv & $ & [#Hm r] & $)". iFrame "Hm". iCombine "Hm Hv r " as "r". iExact "r". }
-    2: { by apply: rec_heap_inj_call_mono. }
+    2: { by apply: rec_heap_bij_call_mono. }
     iSatClear. intros n'' wi ws hi'' hs'' rf'' b'' Hn'' Hsat; simpl.
     tstep_s. intros w Heval. iSatStart.
     iIntros "(Hinv & Hw & HINV & (Hsub & Hv & r) & rf)".
-    iDestruct (eval_binop_inj with "Hv Hw") as "[%u [% Hu]]"; first done.
+    iDestruct (eval_binop_bij with "Hv Hw") as "[%u [% Hu]]"; first done.
     iSatStop. tstep_i. split!. eapply Hcont; first by etrans.
     iSatMono. iFrame.
   - simpl. simpl in Hstatic.
@@ -1111,7 +1111,7 @@ Proof.
     tstep_s. intros l v' -> Hlook. iSatStart.
     iIntros "(Hinv & Hv & HINV & (Hsub & r) & rf)".
     destruct vi; try done; simpl.
-    iDestruct (heap_inj_inv_lookup with "Hinv Hv") as "[%w [% #Hw]]"; [done|set_solver|].
+    iDestruct (heap_bij_inv_lookup with "Hinv Hv") as "[%w [% #Hw]]"; [done|set_solver|].
     iSatStop. tstep_i. split!. eapply Hcont; first by etrans.
     iSatMono. iFrame. iFrame "Hw".
   - simpl. simpl in Hstatic. eapply andb_True in Hstatic as [Hstatic1 Hstat2].
@@ -1120,13 +1120,13 @@ Proof.
       iSatClear. intros n' vi vs hi' hs' rf' b' Hn' Hsat; simpl.
     apply: IH2; simpl; [eauto..|]; last first.
     { iSatMono. iIntros "($ & #Hv & $ & (#Hm & r) & $)". iFrame "Hm". iCombine "Hm Hv r " as "r". iExact "r". }
-    2: { by apply: rec_heap_inj_call_mono. }
+    2: { by apply: rec_heap_bij_call_mono. }
     iSatClear. intros n'' wi ws hi'' hs'' rf'' b'' Hn'' Hsat; simpl.
     tstep_s. intros w -> Halive. iSatStartBupd.
     iIntros "(Hinv & #Hw & HINV & (Hsub & Hv & r) & rf)".
     destruct vi; try done.
-    iDestruct (heap_inj_inv_alive with "Hinv Hv") as "%"; [done|set_solver|].
-    iMod (heap_inj_inv_update with "Hinv Hv Hw") as "Hinv"; [set_solver|done|]. iModIntro.
+    iDestruct (heap_bij_inv_alive with "Hinv Hv") as "%"; [done|set_solver|].
+    iMod (heap_bij_inv_update with "Hinv Hv Hw") as "Hinv"; [set_solver|done|]. iModIntro.
     iSatStop. tstep_i. split!. eapply Hcont; first by etrans.
     iSatMono. iFrame. iFrame "Hw".
   - simpl. simpl in Hstatic. eapply andb_True in Hstatic as [Hstatic Hstatic2].
@@ -1139,12 +1139,12 @@ Proof.
     destruct vi; try done; simpl. iDestruct "Hv" as "->". iSatStop.
     tstep_i. destruct cond.
     + apply: IH1; simpl; eauto.
-      { by apply: rec_heap_inj_call_mono. }
-      { by apply: rec_heap_inj_return_mono. }
+      { by apply: rec_heap_bij_call_mono. }
+      { by apply: rec_heap_bij_return_mono. }
       iSatMono. iFrame.
     + apply: IH2; simpl; eauto.
-      { by apply: rec_heap_inj_call_mono. }
-      { by apply: rec_heap_inj_return_mono. }
+      { by apply: rec_heap_bij_call_mono. }
+      { by apply: rec_heap_bij_return_mono. }
       iSatMono. iFrame.
   - simpl. simpl in Hstatic. eapply andb_True in Hstatic as [Hstatic1 Hstatic2].
     apply: IH1; simpl; [eauto..|]; last first.
@@ -1153,17 +1153,17 @@ Proof.
     tstep_s. tstep_i. rewrite -!subst_subst_map_delete.
     apply: IH2; simpl; eauto.
     { set_solver. }
-    { by apply: rec_heap_inj_call_mono. }
-    { by apply: rec_heap_inj_return_mono. }
+    { by apply: rec_heap_bij_call_mono. }
+    { by apply: rec_heap_bij_return_mono. }
     iSatMono. iIntros "(Hinv & Hv & HINV & (Hsub & r) & rf)". iFrame.
     iApply (big_sepM2_insert_2 with "[Hv]"); by iFrame.
   - simpl. simpl in Hstatic. eapply andb_True in Hstatic as [Hstatic1 Hstatic2].
     apply: IH; simpl; [eauto..|]; last first.
     { iSatMono. iIntros "($ & #Hm & $ & r & $)". iFrame "Hm". iCombine "Hm r" as "r". iExact "r". }
     iSatClear. intros n' vi vs hi' hs' rf' b' Hn' Hsat; simpl.
-    apply: (rec_heap_inj_sim_call_bind args nil nil); simpl; eauto.
+    apply: (rec_heap_bij_sim_call_bind args nil nil); simpl; eauto.
     + iSatMono. iIntros!. iFrame. iAccu.
-    + by apply: rec_heap_inj_call_mono.
+    + by apply: rec_heap_bij_call_mono.
     + clear Hsat vs hi' hs' b' rf'. intros vs ws hi' hs' b' n'' rf' f' Hn'' Hsat'.
       apply: Hcall; simpl; eauto.
       * by etrans.
@@ -1181,14 +1181,14 @@ Proof.
   - done.
 Qed.
 
-Lemma rec_heap_inj_refl fns:
-  trefines (rec_mod fns) (rec_heap_inj (fds_init_heap (fd_static_vars <$> fns)) (rec_mod fns)).
+Lemma rec_heap_bij_refl fns:
+  trefines (rec_mod fns) (rec_heap_bij (fds_init_heap (fd_static_vars <$> fns)) (rec_mod fns)).
 Proof.
-  pose (INV := ([∗ map] f↦fn∈fns, [∗ list] l ∈ static_locs f (fd_static_vars fn), loc_in_inj l l)%I).
-  apply: (rec_heap_inj_proof INV).
+  pose (INV := ([∗ map] f↦fn∈fns, [∗ list] l ∈ static_locs f (fd_static_vars fn), loc_in_bij l l)%I).
+  apply: (rec_heap_bij_proof INV).
   { done. } { naive_solver. } {
     rewrite /INV. iIntros (??) "Hinit Hinv".
-    iMod (heap_inj_inv_share_inits with "Hinv Hinit"). by rewrite big_sepM_fmap.
+    iMod (heap_bij_inv_share_inits with "Hinv Hinit"). by rewrite big_sepM_fmap.
   }
   move => n K1 K2 f fn1 fn2 vs1 v2 h1 h2 r rf ????? Hcall Hret. simplify_eq.
   rewrite !subst_l_subst_map //.
@@ -1199,9 +1199,9 @@ Proof.
   have Hlen2 := (heap_alloc_list_length _ _ _ _ ltac:(done)).
   rewrite length_fmap in Hlen1, Hlen2.
   rewrite /subst_static !subst_l_subst_map ?length_fmap ?length_imap ?length_fmap -?subst_map_subst_map //.
-  apply: (rec_heap_inj_sim_refl_static INV); last first.
+  apply: (rec_heap_bij_sim_refl_static INV); last first.
   - iSatMonoBupd. iIntros "(? & Hvs & #HINV & r & $)".
-    iMod (heap_inj_inv_alloc_list with "[$]") as "[$ Hl]"; [done..|iDestruct "Hl" as "#Hl"].
+    iMod (heap_bij_inv_alloc_list with "[$]") as "[$ Hl]"; [done..|iDestruct "Hl" as "#Hl"].
     iModIntro.
     rewrite -!list_to_map_app. iFrame "HINV".
     iCombine "Hl r" as "r". iSplitR "r"; [| iAccu].
@@ -1217,7 +1217,7 @@ Proof.
     tstep_s => hs' Hfrees.
     tstep_i.
     iSatStartBupd. iIntros!.
-    iMod (heap_inj_inv_free_list with "[$] [$]") as (??) "?"; [done|..]; last (iModIntro; iSatStop; split!; [done|]).
+    iMod (heap_bij_inv_free_list with "[$] [$]") as (??) "?"; [done|..]; last (iModIntro; iSatStop; split!; [done|]).
     all: rewrite ?snd_zip ?fst_zip ?length_fmap //; try lia.
     apply: Hret; [done|].
     iSatMono. iFrame.
@@ -1227,10 +1227,10 @@ Qed.
 
 (** ** Adequacy *)
 
-Lemma rec_heap_inj_rec_closed hinit bs m :
+Lemma rec_heap_bij_rec_closed hinit bs m :
   hinit ⊆ bs →
   let h := (heap_from_blocks bs) in
-  trefines (rec_closed h (rec_heap_inj hinit m)) (rec_closed h m).
+  trefines (rec_closed h (rec_heap_bij hinit m)) (rec_closed h m).
 Proof.
   move => Hh h.
   apply tsim_implies_trefines => /= n.
@@ -1238,7 +1238,7 @@ Proof.
           '(σm1, (σf, σ1, (pp, _, r)), σc1)
           '(σm2, σ2, σc2),
            ∃ rr, r = uPred_shrink rr ∧ σ1 = σ2 ∧ σc1 = σc2 ∧
-             ((σc1 = RCStart h ∧ σf = SMFilter ∧ pp = PPOutside ∧ σm1 = σm2 ∧ σm2 = SMFilter ∧ rr = rec_heap_inj_init hinit) ∨
+             ((σc1 = RCStart h ∧ σf = SMFilter ∧ pp = PPOutside ∧ σm1 = σm2 ∧ σm2 = SMFilter ∧ rr = rec_heap_bij_init hinit) ∨
               ( ((∃ e, σf = SMProgRecv e ∧ σm2 = SMProgRecv e) ∨ (σf = SMProg ∧ σm2 = SMProg)
                  ) ∧ σm1 = SMProg ∧ σc1 = RCRunning ∧ pp = PPInside))
                              ). }
@@ -1251,7 +1251,7 @@ Proof.
     tstep_s. eexists (Some (SMEReturn _)). split!. apply: steps_spec_step_end; [econs|] => ??. simplify_eq/=.
     tstep_i => ??; simplify_eq/=.
     tstep_i. eexists (ValNum <$> vs), h. split!.
-    { apply: satisfiable_mono; [by apply (heap_inj_inv_init bs)|]. iIntros "[$ [Hi Hs]]".
+    { apply: satisfiable_mono; [by apply (heap_bij_inv_init bs)|]. iIntros "[$ [Hi Hs]]".
       iSplitL.
       - iSplitL "Hi"; by iApply big_sepM_subseteq.
       - iSplitL; [|iAccu]. rewrite big_sepL2_fmap_l big_sepL2_fmap_r. iApply big_sepL2_intro; [done|].
@@ -1299,40 +1299,40 @@ Proof.
       tstep_i. apply: steps_impl_step_end => ???. inv_all @m_step.
 Qed.
 
-(** ** [rec_heap_inj] is adequate wrt. contextual refinement *)
+(** ** [rec_heap_bij] is adequate wrt. contextual refinement *)
 (** Follows from the lemmas above. *)
-Lemma rec_heap_inj_trefines_implies_ctx_refines fnsi fnss :
+Lemma rec_heap_bij_trefines_implies_ctx_refines fnsi fnss :
   dom fnsi = dom fnss →
   fd_static_vars <$> fnsi = fd_static_vars <$> fnss →
-  trefines (rec_mod fnsi) (rec_heap_inj (fds_init_heap (fd_static_vars <$> fnss)) (rec_mod fnss)) →
+  trefines (rec_mod fnsi) (rec_heap_bij (fds_init_heap (fd_static_vars <$> fnss)) (rec_mod fnss)) →
   rec_ctx_refines fnsi fnss.
 Proof.
   move => Hdom Hs Href C HC. rewrite /rec_syn_link map_difference_union_r (map_difference_union_r fnss).
   etrans. 2: {
-    by apply (rec_heap_inj_rec_closed (fds_init_heap (fd_static_vars <$> fnss ∪ C ∖ fnss))).
+    by apply (rec_heap_bij_rec_closed (fds_init_heap (fd_static_vars <$> fnss ∪ C ∖ fnss))).
   }
   rewrite !map_fmap_union Hs. rewrite {1}(map_difference_eq_dom_L C fnsi fnss) //.
   apply seq_map_mod_trefines. { apply _. } { apply _. }
   etrans. { apply rec_syn_link_refines_link. apply map_disjoint_difference_r'. }
-  etrans. { eapply rec_link_trefines. 1,2: apply _. 1: done. 1: apply rec_heap_inj_refl. }
-  etrans. { apply rec_heap_inj_combine. 1,2: apply _. 2: done.
+  etrans. { eapply rec_link_trefines. 1,2: apply _. 1: done. 1: apply rec_heap_bij_refl. }
+  etrans. { apply rec_heap_bij_combine. 1,2: apply _. 2: done.
             apply fds_init_heap_disj. apply map_disjoint_fmap.
             rewrite (map_difference_eq_dom_L C fnsi fnss) //. apply map_disjoint_difference_r'. }
   rewrite fds_init_heap_union. 2: { apply map_disjoint_fmap. apply map_disjoint_difference_r'. }
   rewrite {1}(map_difference_eq_dom_L C fnsi fnss) //.
-  apply rec_heap_inj_trefines. 1: apply _.
+  apply rec_heap_bij_trefines. 1: apply _.
   etrans. 2: { apply rec_link_refines_syn_link. apply map_disjoint_difference_r'. }
   rewrite !dom_difference_L Hdom.
   erewrite map_difference_eq_dom_L => //.
   apply _.
 Qed.
 
-(** * Exercising [rec_heap_inj] *)
-Module rec_heap_inj_example.
+(** * Exercising [rec_heap_bij] *)
+Module rec_heap_bij_example.
 
 Local Open Scope Z_scope.
 
-Definition inj_alloc : fndef := {|
+Definition bij_alloc : fndef := {|
   fd_args := [];
   fd_vars := [("tmp", 1)];
   fd_static_vars := [];
@@ -1342,7 +1342,7 @@ Definition inj_alloc : fndef := {|
   fd_static := I;
 |}.
 
-Definition inj_alloc_opt : fndef := {|
+Definition bij_alloc_opt : fndef := {|
   fd_args := [];
   fd_vars := [];
   fd_static_vars := [];
@@ -1351,11 +1351,11 @@ Definition inj_alloc_opt : fndef := {|
   fd_static := I;
 |}.
 
-Lemma inj_alloc_opt_refines :
-  trefines (rec_mod (<["f" := inj_alloc_opt]> ∅))
-           (rec_heap_inj ∅ (rec_mod (<["f" := inj_alloc]> ∅))).
+Lemma bij_alloc_opt_refines :
+  trefines (rec_mod (<["f" := bij_alloc_opt]> ∅))
+           (rec_heap_bij ∅ (rec_mod (<["f" := bij_alloc]> ∅))).
 Proof.
-  apply: (rec_heap_inj_proof True). { compute_done. }
+  apply: (rec_heap_bij_proof True). { compute_done. }
   { move => ??. setoid_rewrite lookup_insert_Some. setoid_rewrite lookup_empty. naive_solver. }
   { iIntros!. by iFrame. }
   move => n K1 K2 f fn1 fn2 vs1 vs2 h1 h2 r rf Hf1 ???? Hcall Hret.
@@ -1368,13 +1368,13 @@ Proof.
   have ? : heap_is_fresh h2 l by apply (heap_fresh_is_fresh ∅). clearbody l.
   apply: Hcall; [done|econs|econs|..].
   { iSatMonoBupd. iIntros!. iFrame.
-    iMod (heap_inj_inv_alloc_s _ _ l with "[$]") as "[? ?]"; [done|].
-    iMod (heap_inj_inv_update_in_block_s with "[$] [$]") as "[$ ?]"; [done|].
+    iMod (heap_bij_inv_alloc_s _ _ l with "[$]") as "[? ?]"; [done|].
+    iMod (heap_bij_inv_update_in_block_s with "[$] [$]") as "[$ ?]"; [done|].
     iModIntro. iAccu. }
   iSatClear.
   move => v1'' v2'' h1'' h2'' rf'' ? /=.
   iSatStart. simplify_eq/=. iIntros!.
-  iDestruct (heap_inj_inv_lookup_block_s with "[$] [$]") as %Hl.
+  iDestruct (heap_bij_inv_lookup_block_s with "[$] [$]") as %Hl.
   iSatStop.
   tstep_i. tstep_i. split!.
   tstep_s.
@@ -1382,16 +1382,16 @@ Proof.
   tstep_s => ?[? [? ?]]. simplify_eq.
   apply Hret; [done|].
   iSatMonoBupd.
-  iMod (heap_inj_inv_free_s with "[$] [$]") as "[$ ?]".
+  iMod (heap_bij_inv_free_s with "[$] [$]") as "[$ ?]".
   iModIntro. by iFrame.
 Qed.
 
 
-Lemma inj_alloc_ctx_refines :
-  rec_ctx_refines (<["f" := inj_alloc_opt]> ∅) (<["f" := inj_alloc]> ∅).
+Lemma bij_alloc_ctx_refines :
+  rec_ctx_refines (<["f" := bij_alloc_opt]> ∅) (<["f" := bij_alloc]> ∅).
 Proof.
-  apply: rec_heap_inj_trefines_implies_ctx_refines; [compute_done..|].
-  have -> : (fds_init_heap (fd_static_vars <$> <["f":=inj_alloc]> ∅)) = ∅ by compute_done.
-  apply inj_alloc_opt_refines.
+  apply: rec_heap_bij_trefines_implies_ctx_refines; [compute_done..|].
+  have -> : (fds_init_heap (fd_static_vars <$> <["f":=bij_alloc]> ∅)) = ∅ by compute_done.
+  apply bij_alloc_opt_refines.
 Qed.
-End rec_heap_inj_example.
+End rec_heap_bij_example.
