dimsum_examples/rec_heap_bij.v
@@ -7,7 +7,7 @@ From dimsum.examples Require Import rec.
 
 Set Default Proof Using "Type".
 
-(** * THIS FILE IS OBSOLETE! USE rec_heap_inj INSTEAD! *)
+(** * THIS FILE IS OBSOLETE! USE rec_heap_bij2 INSTEAD! *)
 
 (** * rec_heap_bij *)
 (** [rec_heap_bij] allows transformations of memory when proving a
